steel/Learn.Steel.DLList.Derived.fst
@@ -1,7 +1,5 @@
 module Learn.Steel.DLList.Derived
 
-module T   = FStar.Tactics
-
 #set-options "--ifuel 1 --fuel 1"
 
 (*** Operations on [dllist_sel_t] *)
@@ -46,11 +44,12 @@ let elim_dllist_nil (#opened : Mem.inames) (p : list_param) (entry exit : ref p.
 
 let intro_dllist_cons (#opened : Mem.inames) (p : list_param) (r0 r1 : ref p.r) (len : nat) (r2 : ref p.r)
   =
-    let c_0 = gget (vcell p r0)                    in
+    let c0  = gget (vcell p r0)                    in
+    let c_0 = (p.cell r0).cl_f c0                  in
     let sl1 = gget (dllist p r1 len r2)            in
     let sl0 = dll_cons #p #r0 #r1 #len #r2 c_0 sl1 in
     change_slprop (vcell p r0 `star` dllist p r1 len r2) (dllist p r0 (len+1) r2)
-      (G.reveal c_0, G.reveal sl1) sl0
+      (G.reveal c0, G.reveal sl1) sl0
       (fun m -> dllist_cons_interp p r0 len r2 m; dllist_cons_sel_eq p r0 len r2 m)
 
 let elim_dllist_cons (#opened : Mem.inames) (p : list_param) (r0 : ref p.r) (len : nat) (r2 : ref p.r)
@@ -61,9 +60,10 @@ let elim_dllist_cons (#opened : Mem.inames) (p : list_param) (r0 : ref p.r) (len
     change_slprop_rel_with_cond
       (dllist p r0 (len+1) r2) (vcell p r0 `star` dllist p r1 len r2)
       (fun sl0' -> sl0' == G.reveal sl0)
-      (fun _ (c_0, sl1) ->
+      (fun _ (c0, sl1) ->
+        let c_0 = (p.cell r0).cl_f c0            in
         let sl1 : dllist_sel_t p r1 len r2 = sl1 in
-        (p.cell r0).get_ref c_0 Forward == r1 /\ sl1.dll_prv == r0 /\
+        c_0.cl_nxt == r1 /\ sl1.dll_prv == r0 /\
         G.reveal sl0 == dll_cons #p #r0 #r1 #len #r2 c_0 sl1)
       (fun m -> dllist_cons_interp p r0 len r2 m; dllist_cons_sel_eq p r0 len r2 m);
     r1
@@ -94,7 +94,7 @@ let rec intro_dllist_append
       let len0' = len0 - 1 in
       dllist_rew_len p r0 len0 (len0'+1) r1;
       let r0' = elim_dllist_cons p r0 len0' r1 in
-      let c   = gget (vcell p r0)              in
+      let c   = gget_cl p r0                   in
       let sl0 = gget (dllist p r0' len0' r1)   in
       let sl1 = gget (dllist p r2  len1  r3)   in
       intro_dllist_append p r0' len0' r1 r2 len1 r3;
@@ -125,7 +125,7 @@ let rec elim_dllist_append
       let len0' = len0 - 1 in
       dllist_rew_len p r0 (len0+len1) ((len0'+len1)+1) r3;
       let r0' : G.erased (ref p.r) = elim_dllist_cons p r0 (len0'+len1) r3 in
-      let c0 = gget (vcell p r0) in
+      let c0 = gget_cl p r0 in
       let sl' : G.erased (dllist_sel_t p r0' (len0'+len1) r3) = gget (dllist p r0' (len0'+len1) r3) in
       dll_tail_append sl0 sl1;
       let sl0' : dllist_sel_t p r0' len0' r1 = U.cast _ (dll_tail sl0) in
@@ -195,7 +195,7 @@ let dllist_read_next
   =
     (**) dllist_rew_len p r0 len (len'+1) r2;
     (**) let g_r1 : G.erased (ref p.r) = elim_dllist_cons p r0 len' r2 in
-    let r1 : ref p.r = (p.cell r0).read_ref Forward in
+    let r1 : ref p.r = (p.cell r0).read_nxt () in
     (**) assert (G.reveal g_r1 == r1);
     (**) change_equal_slprop (dllist p g_r1 len' r2)
     (**)                     (dllist p r1   len' r2);
@@ -208,38 +208,39 @@ let dllist_splitOn
       (p : list_param) (r0 : ref p.r) (len : G.erased nat) (r1 : G.erased (ref p.r))
       (r : ref p.r) (i : G.erased (Fin.fin len))
   =
-    let sl    : G.erased (dllist_sel_t p r0 len r1) = gget (dllist p r0 len r1) in
-    let sls   : G.erased (rs0 : ref p.r & rs1 : ref p.r & dllist_sel_t p r0 i rs0 & dllist_sel_t p rs1 (len-i) r1)
-              = G.hide (dll_splitAt i sl)          in
-    let len1  : G.erased nat = G.hide (len-i)        in
-    let g_rs0 : G.erased (ref p.r) = G.hide sls._1 in
-    assert (sls._2 == r);
-    let sl0   : G.erased (dllist_sel_t p r0 i g_rs0) = G.hide sls._3 in
-    let sl1   : G.erased (dllist_sel_t p r len1 r1)  = G.hide sls._4 in
-    dll_splitAt_append i sl;
-    change_equal_slprop (dllist p r0   len    r1)
-                        (dllist p r0 (i+len1) r1);
-    elim_dllist_append p r0 i g_rs0 r len1 r1 sl0 sl1;
-    let len2 : G.erased nat = G.hide (len1-1)       in
+    (**) let sl    : G.erased (dllist_sel_t p r0 len r1) = gget (dllist p r0 len r1) in
+    (**) let len1  : G.erased nat = G.hide (len-i)        in
+    (**) let sls 
+    (**)   : G.erased (rs0 : ref p.r & rs1 : ref p.r & dllist_sel_t p r0 i rs0 & dllist_sel_t p rs1 len1 r1)
+    (**)   = G.hide (dll_splitAt i sl)                  in
+    (**) let g_rs0 : G.erased (ref p.r) = G.hide sls._1 in
+    (**) assert (sls._2 == r);
+    (**) let sl0   : G.erased (dllist_sel_t p r0 i g_rs0) = G.hide sls._3 in
+    (**) let sl1   : G.erased (dllist_sel_t p r len1 r1)  = G.hide sls._4 in
+    (**) dll_splitAt_append i sl;
+    (**) change_equal_slprop (dllist p r0   len    r1)
+    (**)                     (dllist p r0 (i+len1) r1);
+    (**) elim_dllist_append p r0 i g_rs0 r len1 r1 sl0 sl1;
+    (**) let len2 : G.erased nat = G.hide (len1-1)       in
     let rs1 = dllist_read_next p r len1 len2 r1   in
-    let rs0 = (p.cell r).read_ref Backward        in
-    change_equal_slprop (dllist p r0 i g_rs0)
-                        (dllist p r0 i   rs0);
-    let c    = gget (vcell p r)            in
-    let sl1' : G.erased (dllist_sel_t p rs1 len2 r1) = gget (dllist p rs1 len2 r1) in
-    assert (G.reveal sl1 == dll_cons c sl1');
-    assert (dll_tail sl1 == G.reveal sl1');
-    U.assert_by (index sl.dll_sg i == (|r, (p.cell r).get_data c|)) (fun () ->
-      calc (==) {
-        index sl.dll_sg i;
-      == { Ll.splitAt_index i sl.dll_sg }
-        index sl1.dll_sg 0;
-      == { }
-        index (dll_cons c sl1').dll_sg 0;
-      == { U.by_refl () }
-        (|r, (p.cell r).get_data c|);
-      }
-    );
+    let rs0 = (p.cell r).read_prv ()              in
+    (**) change_equal_slprop (dllist p r0 i g_rs0)
+    (**)                     (dllist p r0 i   rs0);
+    (**) let c    = gget_cl p r                        in
+    (**) let sl1' : G.erased (dllist_sel_t p rs1 len2 r1) = gget (dllist p rs1 len2 r1) in
+    (**) assert (G.reveal sl1 == dll_cons c sl1');
+    (**) assert (dll_tail sl1 == G.reveal sl1');
+    (**) U.assert_by (index sl.dll_sg i == (|r, c.cl_data|)) (fun () ->
+    (**)   calc (==) {
+    (**)     index sl.dll_sg i;
+    (**)   == { Ll.splitAt_index i sl.dll_sg }
+    (**)     index sl1.dll_sg 0;
+    (**)   == { }
+    (**)     index (dll_cons c sl1').dll_sg 0;
+    (**)   == { U.by_refl () }
+    (**)     (|r, c.cl_data|);
+    (**)   }
+    (**) );
     return (rs0, rs1)
 #pop-options
 
@@ -249,15 +250,10 @@ let dllist_change_prv_cons
       (p : list_param) (r0 : ref p.r) (len : G.erased nat {len > 0}) (r1 : G.erased (ref p.r))
       (prv : ref p.r)
   =
-    (**) let len' = G.hide (len - 1) in
+    (**) let len' = G.hide (len - 1)             in
     (**) dllist_rew_len p r0 len (len'+1) r1;
     (**) let r0' = elim_dllist_cons p r0 len' r1 in
-    (**) let c0 = gget (vcell p r0) in
-    (p.cell r0).write_ref Backward prv;
-    (**) let c1 = gget (vcell p r0) in
-    (**) assert ((p.cell r0).get_ref c0 Forward == G.reveal r0');
-    (**) assert (G.reveal c1 == (p.cell r0).set_ref c0 Backward prv);
-    (**) assert ((p.cell r0).get_ref c1 Forward == G.reveal r0');
+    (p.cell r0).write_prv prv;
     (**) intro_dllist_cons p r0 r0' len' r1;
     (**) dllist_rew_len p r0 (len'+1) len r1
 
@@ -284,11 +280,10 @@ let dllist_change_nxt_cons
       (p : list_param) (r0 : G.erased (ref p.r)) (len : G.erased nat {len > 0}) (r1 : ref p.r)
       (nxt : ref p.r)
   =
-    (**) let len' = G.hide (len - 1) in
+    (**) let len' = G.hide (len - 1)             in
     (**) dllist_rew_len p r0 len (len'+1) r1;
     (**) let r1' = elim_dllist_snoc p r0 len' r1 in
-    (**) let c0 = gget (vcell p r1) in // necessary for the SMT to see that Backward does not change
-    (p.cell r1).write_ref Forward nxt;
+    (p.cell r1).write_nxt nxt;
     (**) intro_dllist_snoc p r0 len' r1' r1;
     (**) dllist_rew_len p r0 (len'+1) len r1
 
