steel/Learn.Steel.DLList.Data.fsti
@@ -12,18 +12,19 @@ open Learn.Steel.DLList.Param
 
 #set-options "--fuel 1 --ifuel 1"
 
-let sg_entry (#p : list_param) (l : list (cell_t p)) (nxt : ref p.r) : ref p.r =
+let sg_entry (#p : list_param) (l : list (rcell_t p)) (nxt : ref p.r) : ref p.r =
   match l with
   | [] -> nxt
   | hd :: _ -> hd._1
 
-let sg_exit  (#p : list_param) (prv : ref p.r) (l : list (cell_t p)) : ref p.r =
+let sg_exit  (#p : list_param) (prv : ref p.r) (l : list (rcell_t p)) : ref p.r =
   if Cons? l then (last l)._1 else prv
 
 // ALT: dllist_sel_t' + refinement
+// ALT: indexed by prv + entry ?
 noeq
 type dllist_sel_t (p : list_param) (entry : ref p.r) (len : nat) (exit : ref p.r) : Type = {
-  dll_sg  : llist (cell_t p) len;
+  dll_sg  : llist (rcell_t p) len;
   dll_prv : prv : ref p.r { exit  == sg_exit  prv dll_sg };
   dll_nxt : nxt : ref p.r { entry == sg_entry dll_sg nxt };
 }
@@ -43,15 +44,15 @@ let dll_nil (#p : list_param) (entry : ref p.r) (exit : ref p.r)
     dll_nxt = entry;
   }
 
-/// [r1] should be [(p.cell r0).get_ref c Forward]
+/// [r1] should be [c.cl_nxt]
 let dll_cons
       (#p : list_param) (#r0 #r1 : ref p.r) (#len' : nat) (#r2 : ref p.r)
-      (c : t_of (vcell p r0))
+      (c : cell_t p r0)
       (sl1 : dllist_sel_t p r1 len' r2 {sl1.dll_prv == r0})
   : GTot (dllist_sel_t p r0 (len' + 1) r2)
   = {
-    dll_sg  = (|r0, (p.cell r0).get_data c|) :: sl1.dll_sg;
-    dll_prv = (p.cell r0).get_ref c Backward;
+    dll_sg  = (|r0, c.cl_data|) :: sl1.dll_sg;
+    dll_prv = c.cl_prv;
     dll_nxt = sl1.dll_nxt;
   }
 
@@ -86,18 +87,18 @@ val dllist_nil_interp (p : list_param) (entry : ref p.r) (exit : ref p.r) (m : M
 val dllist_cons_interp (p : list_param) (entry : ref p.r) (len : nat) (exit : ref p.r) (m : Mem.mem)
   : Lemma (Mem.interp (hp_of (dllist p entry (len + 1) exit)) m
          <==> Mem.interp (hp_of (vcell p entry)) m /\
-           (let c = sel_of (vcell p entry) m in
-            let entry' = (p.cell entry).get_ref c Forward in
+           (let      c = (p.cell entry).cl_f (sel_of (vcell p entry) m) in
+            let entry' = c.cl_nxt                                       in
             Mem.interp (hp_of (vcell p entry) `Mem.star` hp_of (dllist p entry' len exit)) m /\
            (let sl1 : dllist_sel_t p entry' len exit
-                    = sel_of (dllist p entry' len exit) m in
+                    = sel_of (dllist p entry' len exit) m               in
             sl1.dll_prv == entry)))
 
 val dllist_cons_sel_eq
       (p : list_param) (entry : ref p.r) (len : nat) (exit : ref p.r) (m : Mem.mem)
   : Lemma (requires Mem.interp (hp_of (dllist p entry (len + 1) exit )) m)
           (ensures (dllist_cons_interp p entry len exit m;
-                    let c = sel_of (vcell p entry) m              in
-                    let entry' = (p.cell entry).get_ref c Forward in
-                    let sl1 = sel_of (dllist p entry' len exit) m in
+                    let c      = (p.cell entry).cl_f (sel_of (vcell p entry) m) in
+                    let entry' = c.cl_nxt                                       in
+                    let sl1    = sel_of (dllist p entry' len exit) m            in
                     sel_of (dllist p entry (len + 1) exit) m == dll_cons #p #entry #entry' #len #exit c sl1))
