steel/Learn.Steel.DLList.Test.fst
@@ -1,0 +1,25 @@
+module Learn.Steel.DLList.Test
+
+module U32 = FStar.UInt32
+
+open FStar.Ghost
+open Steel.Effect
+open Steel.Reference
+open Learn.Steel.DLList
+
+noeq
+type cell0 = {
+  prv : ref cell0;
+  nxt : ref cell0;
+  data0 : bool;
+  data1 : U32.t;
+}
+
+inline_for_extraction noextract
+let p0 : list_param
+  = list_param_of_vptr cell0 (bool & U32.t)
+      (fun s -> {cl_prv = s.prv; cl_nxt = s.nxt; cl_data = (s.data0, s.data1)})
+      (fun s prv -> {s with prv})
+      (fun s nxt -> {s with nxt})
+
+let p0_remove = remove p0
