steel/Learn.Steel.DLList.fst
@@ -2,4 +2,5 @@ module Learn.Steel.DLList
 
 include Learn.Steel.DLList.Param
 include Learn.Steel.DLList.Data
+include Learn.Steel.DLList.Impl
 
